@prefix schema: <http://schema.org/> .
@prefix adms: <http://www.w3.org/ns/adms#> .
@prefix owl: <http://www.w3.org/2002/07/owl#> .
@prefix org: <http://www.w3.org/ns/org#> .
@prefix xsd: <http://www.w3.org/2001/XMLSchema#> .
@prefix skosthes: <http://purl.org/iso25964/skos-thes#> .
@prefix rdfs: <http://www.w3.org/2000/01/rdf-schema#> .
@prefix qb: <http://purl.org/linked-data/cube#> .
@prefix cv: <http://data.europa.eu/m8g> .
@prefix dct: <http://purl.org/dc/terms/> .
@prefix rdf: <http://www.w3.org/1999/02/22-rdf-syntax-ns#> .
@prefix doap: <http://usefulinc.com/ns/doap#> .
@prefix sh: <http://www.w3.org/ns/shacl#> .
@prefix vann: <http://purl.org/vocab/vann/> .
@prefix dcat: <http://www.w3.org/ns/dcat#> .
@prefix euvoc: <http://publications.europa.eu/ontology/euvoc#> .
@prefix prov: <http://www.w3.org/ns/prov#> .
@prefix foaf: <http://xmlns.com/foaf/0.1/> .
@prefix dc: <http://purl.org/dc/elements/1.1/> .
@prefix skos: <http://www.w3.org/2004/02/skos/core#> .
@prefix skosxl: <http://www.w3.org/2008/05/skos-xl#> .

<http://data.europa.eu/m8g/evap/2.0.0> a owl:Ontology;
  vann:preferredNamespaceURI "http://data.europa.eu/m8g/evap";
  vann:preferredNamespacePrefix "evap"@en;
  dct:title "EV-AP"@en;
  dct:description "The Core Public Service Vocabulary Application Profile (CPSV-AP) is a reusable and extensible data specification used for harmonising the way public services are described in a machine-readable format. CPSV-AP captures fundamental characteristics of a public service, such as the name, description, competent public organisation, output, etc. Public administrations and service providers can therefore use this approach to describe their services and guarantee a level of cross-domain and cross-border interoperability at European, national and local level."@en;
  owl:versionIRI <http://data.europa.eu/m8g/evap/2.0.0>;
  owl:versionInfo "2.0.0"@en;
  dct:created "2023-05-03"^^xsd:date;
  dct:creator <http://publications.europa.eu/resource/authority/corporate-body/DIGIT>;
  dct:license <https://creativecommons.org/licenses/by/4.0/> .

<http://www.w3.org/ns/legal#LegalEntity> a owl:Class;
  rdfs:comment "A self-empoyed person, company, or organization that has legal rights and obligations."@en;
  rdfs:label "Legal Entity"@en;
  vann:usageNote "A Legal Entity able to transact business, typically registered with a body able to confer legal status such as a national business register. It is able to trade, is legally liable for its actions, accounts, tax affairs etc. This makes Legal Entities distinct from the concept of organisations, groups or sole traders. Many organisations exist that are not Legal Entities, yet to the outside world they have staff, hierarchies, locations etc. Other organisations exist that are an umbrella for several Legal Entities (universities are often good examples of this). This vocabulary is concerned solely with registered Legal Entities and does not attempt to cover all possible trading bodies."@en;
  rdfs:subClassOf org:FormalOrganization .

<http://www.w3.org/ns/legal#legalName> a owl:DatatypeProperty;
  rdfs:comment "The name under which the Legal Entity is legally registered."@en;
  rdfs:label "legal name"@en;
  vann:usageNote """The legal name is different from the alternative (trade) name which is a pseudonym used by companies that do not operate under their registered company name.
A business might have more than one legal name, particularly in countries with more than one official language. In such cases, and where the encoding technology allows, the language of the string should be identified."""@en;
  rdfs:range rdf:langString .

<http://data.europa.eu/m8g/contactPoint> a owl:ObjectProperty;
  rdfs:comment "The main contact information of the resource."@en;
  rdfs:label "contact point"@en;
  vann:usageNote "Usually a phone number and e-mail address. Other contact methods may be included, including online contact information, but this is conceptually distinct from the organization's homepage that may or may not provide contact information."@en;
  rdfs:range <http://data.europa.eu/m8g/ContactPoint> .

<http://data.europa.eu/m8g/registeredAddress> a owl:ObjectProperty;
  rdfs:comment "The address at which the Legal Entity is legally registered."@en;
  rdfs:label "registered address"@en;
  vann:usageNote "In almost all jurisdictions, Legal Entities must register a public address. This may or may not be the actual address at which the Legal Entity does its business, it is commonly the address of their lawyer or accountant, but it is the address to which formal communications can be sent. The registered address property points to the Address of the Registered Site. This property can be seen as a shorthand for this property path."@en;
  rdfs:range <http://www.w3.org/ns/locn#Address> .

<http://www.w3.org/ns/locn#Address> a owl:Class;
  rdfs:comment "A spatial object that in a human-readable way identifies a fixed location."@en;
  rdfs:label "Address"@en;
  vann:usageNote """An \"address representation\" as conceptually defined by the <a href=\"https://inspire-regadmin.jrc.ec.europa.eu/dataspecification/ScopeObjectDetail.action?objectDetailId=9353\">INSPIRE Address Representation data type</a>: \"Representation of an address spatial object for use in external application schemas that need to include the basic, address information in a readable way.\".
<br/><br/>
The representation of Addresses varies widely from one country's postal system to another. Even within countries, there are almost always examples of Addresses that do not conform to the stated national standard. However, <a href=\"https://www.iso.org/standard/61710.html\">ISO 19160-1</a> provides a method through which different Addresses can be converted from one conceptual model to another.
<br/><br/>
This specification was heavily based on the INSPIRE Address Representation data type. It is noteworthy that if an Address is provided using the detailed breakdown suggested by the properties for this class, then it will be INSPIRE-conformant. To this very granular set of properties, we add two further properties:
<br/><br/>
- full address (the complete address as a formatted string)<br/>
- addressID (a unique identifier for the address).
The first of these allows publishers to simply provide the complete Address as one string, with or without formatting. This is analogous to <a href=\"https://www.w3.org/TR/vcard-rdf/#d4e953\">vCard's label property</a>.
<br/><br/>
The addressID is part of the INSPIRE guidelines and provides a hook that can be used to link the Address to an alternative representation, such as vCard or OASIS xAL.
<br/><br/>
This class belongs to <a href=\"https://semiceu.github.io/Core-Location-Vocabulary/releases/2.00/#Address\">Core Location Vocabulary</a>"""@en .

<http://www.w3.org/ns/locn#addressArea> a owl:DatatypeProperty;
  rdfs:comment "The name of a geographic area that groups Addresses."@en;
  rdfs:label "address area"@en;
  vann:usageNote "This would typically be part of a city, a neighbourhood or village, e.g. Montmartre. Address area is not an administrative unit."@en;
  rdfs:range rdf:langString .

<http://www.w3.org/ns/locn#addressId> a owl:DatatypeProperty;
  rdfs:comment "A globally unique identifier for each instance of an Address."@en;
  rdfs:label "address ID"@en;
  vann:usageNote """The concept of adding a globally unique identifier for each instance of an address is a crucial part of the INSPIRE data spec. A number of EU countries have already implemented an ID (a UUID) in their Address Register/gazetteer, among them Denmark. OASIS xAL also includes an address identifier. It is the address Identifier that allows an address to be represented in a format other than INSPIRE whilst remaining conformant to the Core Vocabulary.
<br/><br/>
The INSPIRE method of representing addresses is very detailed, designed primarily for use in databases of addresses. Whilst data that is published in full conformance with the INSPIRE data structure can be made available using the Core Location Vocabulary the reverse is not true since the Core Vocabulary allows much greater flexibility.
<br/><br/>
Many datasets that include address data as one piece of information about something else are likely to have that data in simpler formats. These might be tailored to the specific need of the dataset, follow a national norm, or make use of a standard like vCard.
<br/><br/>
To provide maximum flexibility in the Core Vocabulary, whilst remaining interoperable with INSPIRE Address Guidelines (which EU Member States are obliged to use), the Core Location Vocabulary provides the extra property of full address and makes use of INSPIRE's addressID.
<br/><br/>
The datatype of addressID is indicated as Literal (keeping backward compatibility with the old W3C specification) that can be typed differently, see <a href=\"https://www.w3.org/TR/rdf11-concepts/#section-Graph-Literal\">more</a>."""@en;
  rdfs:range rdfs:Literal .

<http://www.w3.org/ns/locn#adminUnitL1> a owl:DatatypeProperty;
  rdfs:comment "The name of the uppermost level of the address, almost always a country."@en;
  rdfs:label "administrative unit level 1"@en;
  vann:usageNote "Best practice is to use the ISO 3166-1 code but if this is inappropriate for the context, country names should be provided in a consistent manner to reduce ambiguity. For example, either write 'France' or 'FRA' consistently throughout the dataset and avoid mixing the two. The <a href=\"https://op.europa.eu/en/web/eu-vocabularies/dataset/-/resource?uri=http://publications.europa.eu/resource/dataset/country\">Country controlled vocabulary</a> from the Publications Office can be reused for this."@en;
  rdfs:range rdf:langString .

<http://www.w3.org/ns/locn#adminUnitL2> a owl:DatatypeProperty;
  rdfs:comment "The name of a secondary level/region of the address, usually a county, state or other such area that typically encompasses several localities."@en;
  rdfs:label "administrative unit level 2"@en;
  vann:usageNote "Values could be a region or province, more granular than level 1."@en;
  rdfs:range rdf:langString .

<http://www.w3.org/ns/locn#fullAddress> a owl:DatatypeProperty;
  rdfs:comment "The complete address written as a string."@en;
  rdfs:label "full address"@en;
  vann:usageNote "Use of this property is recommended as it will not suffer any misunderstandings that might arise through the breaking up of an address into its component parts. This property is analogous to vCard's label property but with two important differences: (1) formatting is not assumed so that, unlike vCard label, it may not be suitable to print this on an address label, (2) vCard's label property has a domain of vCard Address; the fullAddress property has no such restriction. An example of a full address is \"Champ de Mars, 5 Avenue Anatole France, 75007 Paris, France\"."@en;
  rdfs:range rdf:langString .

<http://www.w3.org/ns/locn#locatorDesignator> a owl:DatatypeProperty;
  rdfs:comment "A number or sequence of characters that uniquely identifies the locator within the relevant scope."@en;
  rdfs:label "locator designator"@en;
  vann:usageNote """In simpler terms, this is the building number, apartment number, etc. For an address such as \"Flat 3, 17 Bridge Street\", the locator is \"flat 3, 17\".
<br/><br/>
The datatype of locatorDesignator is indicated as Literal (keeping backward compatibility with the old W3C specification) that can be typed differently, see <a href=\"https://www.w3.org/TR/rdf11-concepts/#section-Graph-Literal\">more</a>."""@en;
  rdfs:range rdfs:Literal .

<http://www.w3.org/ns/locn#locatorName> a owl:DatatypeProperty;
  rdfs:comment "Proper noun(s) applied to the real world entity identified by the locator."@en;
  rdfs:label "locator name"@en;
  vann:usageNote """The locator name could be the name of the property or complex, of the building or part of the building, or it could be the name of a room inside a building.
<br/><br/>
The key difference between a locator and a locator name is that the latter is a proper name and is unlikely to include digits. For example, \"Shumann, Berlaymont\" is a meeting room within the European Commission headquarters for which locator name is more appropriate than locator."""@en;
  rdfs:range rdf:langString .

<http://www.w3.org/ns/locn#poBox> a owl:DatatypeProperty;
  rdfs:comment "A location designator for a postal delivery point at a post office, usually a number."@en;
  rdfs:label "post office box"@en;
  vann:usageNote """INSPIRE's name for this is \"postalDeliveryIdentifier\" for which it uses the locator designator property with a type attribute of that name. This vocabulary separates out the Post Office Box for greater independence of technology. An example post office box number is \"9383\".
<br/><br/>
The datatype of poBox is indicated as Literal (keeping backward compatibility with the old W3C specification) that can be typed differently, see <a href=\"https://www.w3.org/TR/rdf11-concepts/#section-Graph-Literal\">more</a>."""@en;
  rdfs:range rdfs:Literal .

<http://www.w3.org/ns/locn#postCode> a owl:DatatypeProperty;
  rdfs:comment "The code created and maintained for postal purposes to identify a subdivision of addresses and postal delivery points."@en;
  rdfs:label "post code"@en;
  vann:usageNote """Post codes are common elements in many countries' postal address systems. One of the many post codes of Paris is for example \"75000\".

The datatype of addressID is indicated as Literal (keeping backward compatibility with the old W3C specification) that can be typed differently, see <a href=\"https://www.w3.org/TR/rdf11-concepts/#section-Graph-Literal\">more</a>."""@en;
  rdfs:range rdfs:Literal .

<http://www.w3.org/ns/locn#postName> a owl:DatatypeProperty;
  rdfs:comment "A name created and maintained for postal purposes to identify a subdivision of addresses and postal delivery points."@en;
  rdfs:label "post name"@en;
  vann:usageNote "Usually a city, for example \"Paris\"."@en;
  rdfs:range rdf:langString .

<http://www.w3.org/ns/locn#thoroughfare> a owl:DatatypeProperty;
  rdfs:comment "The name of a passage or way through from one location to another."@en;
  rdfs:label "thoroughfare"@en;
  vann:usageNote "A thoroughfare is usually a street, but it might be a waterway or some other feature. For example, \"Avenue des Champs-Élysées\"."@en;
  rdfs:range rdf:langString .

<http://www.w3.org/ns/locn#Geometry> a owl:Class;
  rdfs:comment "A shape or form of a Location."@en;
  rdfs:label "Geometry"@en;
  vann:usageNote "This class defines the notion of \"geometry\" at the conceptual level, and it shall be encoded by using different formats (see usage note of the locn:geometry property). Can be a point, line or polygon, expressed using coordinates in some coordinate reference system. We also refer to the Examples section of this specification for a number of different geometry examples expressed in different formats."@en .

<http://data.europa.eu/m8g/coordinates> a owl:DatatypeProperty;
  rdfs:comment "A list of geographic coordinates that define the extent of the Geometry."@en;
  rdfs:label "coordinates"@en;
  vann:usageNote "Can be expressed as longitude, latitude, elevation."@en;
  rdfs:range xsd:string .

<http://data.europa.eu/m8g/geometryType> a owl:ObjectProperty;
  rdfs:comment "The classification of the Geometry."@en;
  rdfs:label "geometry type"@en;
  vann:usageNote "Can be a point, line or polygon."@en;
  rdfs:range skos:Concept .

<http://data.europa.eu/m8g/latitude> a owl:DatatypeProperty;
  rdfs:comment "The geographic coordinate that specifies the north / south position of the Geomerty on the Earth's surface."@en;
  rdfs:label "latitude"@en;
  rdfs:range xsd:string .

<http://data.europa.eu/m8g/longitude> a owl:DatatypeProperty;
  rdfs:comment "The geographic coordinate that specifies the east / west position of the Geometry on the Earth's surface."@en;
  rdfs:label "longitude"@en;
  rdfs:range xsd:string .

<http://www.w3.org/ns/person#Person> a owl:Class;
  rdfs:comment "A individual human being who may be dead or alive, but not imaginary."@en;
  rdfs:label "Person"@en;
  vann:usageNote "The fact that a person in the context of Core Person Vocabulary cannot be imaginary makes person:Person a subclass of both foaf:Person and schema:Person which both cover imaginary characters as well as real people. The Person Class is a subclass of the more general <a href=\"#Agent\">'Agent' class</a>."@en .

foaf:familyName a owl:DatatypeProperty;
  rdfs:comment "The hereditary surname of a family."@en;
  rdfs:label "family name"@en;
  vann:usageNote "Usually referring to a group of people related by blood, marriage or adoption. This attribute also carries prefixes or suffixes which are part of the family name, e.g. \"de Boer\", \"van de Putte\", \"von und zu Orlow\". Multiple family names, such as are commonly found in Hispanic countries, are recorded in the single family name property so that, for example, Miguel de Cervantes Saavedra's family name would be recorded as \"de Cervantes Saavedra\"."@en;
  rdfs:range rdf:langString .

foaf:givenName a owl:DatatypeProperty;
  rdfs:comment "The name(s) that identify the Person within a family with a common surname."@en;
  rdfs:label "given name"@en;
  vann:usageNote "Usually a first name. Given to a person by his or her parents at birth or legally recognised as 'given names' through a formal process. All given names are ordered in one property so that, for example, the given name for Johann Sebastian Bach is \"Johann Sebastian\"."@en;
  rdfs:range rdf:langString .

<http://data.europa.eu/m8g/domicile> a owl:ObjectProperty;
  rdfs:comment "The place that the Person treats as permanent home."@en;
  rdfs:label "domicile"@en;
  rdfs:range <http://www.w3.org/ns/locn#Address> .

<http://data.europa.eu/m8g/owns> a owl:ObjectProperty;
  rdfs:comment "it relates to something belonging to an entity."@en;
  rdfs:label "owns"@en;
  rdfs:range <http://data.europa.eu/m8g/ElectricCar> .

<http://data.europa.eu/m8g/ContactPoint> a owl:Class;
  rdfs:comment "Information (e.g. e-mail address, telephone number) of a person or department through which the user can get in touch with."@en;
  rdfs:label "Contact Point"@en;
  vann:usageNote "The Core Public Organization Vocabulary defines properties for telephone number, e-mail address and opening hours although it is noteworthy that the class is based on schema.org's ContactPoint class (http://schema.org/ContactPoint) that has additional properties that some implementations may find useful."@en .

<http://data.europa.eu/m8g/contactPage> a owl:ObjectProperty;
  rdfs:comment "A web page that could be used to reach out the Contact Point."@en;
  rdfs:label "contact page"@en;
  rdfs:range foaf:Document .

<http://data.europa.eu/m8g/email> a owl:DatatypeProperty;
  rdfs:comment "An electronic address through which the Contact Point can be contacted."@en;
  rdfs:label "has email"@en;
  rdfs:range rdfs:Literal .

<http://data.europa.eu/m8g/telephone> a owl:DatatypeProperty;
  rdfs:comment "A telephone number through which the Contact Point can be contacted."@en;
  rdfs:label "has telephone"@en;
  rdfs:range rdfs:Literal .

<http://data.europa.eu/m8g/generates> a owl:ObjectProperty;
  rdfs:comment "It relates to something that is produced or created."@en;
  rdfs:label "generates"@en;
  rdfs:range <https://smartdatamodels.org/dataModel.Battery/StorageBatteryMeasurement> .

<https://spec.edmcouncil.org/auto/ontology/VS/VehicleSignals/BatterySensor> a owl:Class;
  rdfs:comment "Sensor measuring the capacity of a battery"@en;
  rdfs:label "Battery Sensor"@en;
  rdfs:subClassOf <https://spec.edmcouncil.org/auto/ontology/VS/VehicleSignals/VehicleSensor> .

<http://data.europa.eu/m8g/pluggedTo> a owl:ObjectProperty;
  rdfs:comment "It relates to something physically connected."@en;
  rdfs:label "plugged to"@en;
  rdfs:range <http://data.europa.eu/m8g/StorageBatteryDevice> .

<http://data.europa.eu/m8g/reports> a owl:ObjectProperty;
  rdfs:comment "it relates to something to which information is provided to."@en;
  rdfs:label "reports"@en;
  rdfs:range <http://data.europa.eu/m8g/BatteryManagementSystem> .

<http://data.europa.eu/m8g/CarManufacturer> a owl:Class;
  rdfs:comment "The manufacturer of the vehicle."@en;
  rdfs:label "Car Manufacturer"@en;
  rdfs:subClassOf <http://www.w3.org/ns/legal#LegalEntity>;
  owl:equivalentClass <https://schema.org/manufacturer>, "bamm:io.catenax.vehicle.product_description:2.0.0#OriginalEquipmentManufacturer"@en .

<http://data.europa.eu/m8g/businessPartnerNumber> a owl:DatatypeProperty;
  rdfs:comment "A business partner number of this company."@en;
  rdfs:label "business partner number"@en;
  rdfs:range xsd:string;
  owl:equivalentProperty "urn:bamm:io.catenax.vehicle.product_description:2.0.0#cxBPN"@en .

<http://data.europa.eu/m8g/wmi> a owl:DatatypeProperty;
  rdfs:comment "3-character World Manufacturer Identification (WMI) as defined by ISO 3780"@en;
  rdfs:label "WMI"@en;
  rdfs:range xsd:string;
  owl:equivalentProperty "urn:bamm:io.catenax.vehicle.product_description:2.0.0#wmiCode"@en .

<http://data.europa.eu/m8g/ElectricCar> a owl:Class;
  rdfs:comment "Car that solely uses electric propulsion."@en;
  rdfs:label "Electric Car"@en;
  owl:equivalentClass <https://schema.org/Car>, <https://spec.edmcouncil.org/auto/ontology/VC/VehicleCore/Car>,
    <https://www.w3.org/TR/vsso-core/#Vehicle> .

<http://data.europa.eu/m8g/inletType> a owl:ObjectProperty;
  rdfs:comment "The type of plug this car is equiped with."@en;
  rdfs:label "inletType"@en;
  rdfs:range skos:Concept .

<http://data.europa.eu/m8g/make> a owl:DatatypeProperty;
  rdfs:comment "The make is the brand name used by the car manufacturer."@en;
  rdfs:label "make"@en;
  rdfs:range xsd:string;
  owl:equivalentProperty <https://schema.org/brand> .

<http://data.europa.eu/m8g/model> a owl:DatatypeProperty;
  rdfs:comment "The model of a car is its design, in the context of the manufacturer's range or series of cars."@en;
  rdfs:label "model"@en;
  rdfs:range xsd:string;
  owl:equivalentProperty <https://schema.org/model> .

<http://data.europa.eu/m8g/modelYear> a owl:DatatypeProperty;
  rdfs:comment "The year in which the model has been conceived."@en;
  rdfs:label "model year"@en;
  rdfs:range xsd:gYear;
  owl:equivalentProperty <https://schema.org/productionDate> .

<http://data.europa.eu/m8g/vehicleIdentificationNumber> a owl:DatatypeProperty;
  rdfs:comment "The Vehicle Identification Number (VIN) is a unique serial number used by the automotive industry to identify individual motor vehicles."@en;
  rdfs:label "vehicle identification number"@en;
  rdfs:range xsd:string;
  owl:equivalentProperty <https://schema.org/vehicleIdentificationNumber> .

<http://data.europa.eu/m8g/chargedAt> a owl:ObjectProperty;
  rdfs:comment "The source power to which an electric appliance can get energy from."@en;
  rdfs:label "charged at"@en;
  rdfs:range <https://smartdatamodels.org/dataModel.Transportation/EVChargingStation> .

<http://data.europa.eu/m8g/fuelConsumption> a owl:ObjectProperty;
  rdfs:comment "The fuel used per unit of distance traveled."@en;
  rdfs:label "fuel consumption"@en;
  rdfs:range <http://qudt.org/schema/qudt/QuantityValue>;
  owl:equivalentProperty <https://schema.org/fuelConsumption>, <https://spec.edmcouncil.org/auto/ontology/VC/VehicleCore/fuelConsumption> .

<http://data.europa.eu/m8g/fuelEfficiency> a owl:ObjectProperty;
  rdfs:comment "The distance traveled per unit of fuel used."@en;
  rdfs:label "fuel efficiency"@en;
  rdfs:range <http://qudt.org/schema/qudt/QuantityValue>;
  owl:equivalentProperty <https://schema.org/fuelEfficiency> .

<http://data.europa.eu/m8g/hasManufacturer> a owl:ObjectProperty;
  rdfs:comment "The manufacturer of the vehicle."@en;
  rdfs:label "has manufacturer"@en;
  rdfs:range <http://data.europa.eu/m8g/CarManufacturer>;
  owl:equivalentProperty <https://schema.org/manufacturer> .

dct:hasPart a owl:ObjectProperty;
  rdfs:comment "A related resource that is included either physically or logically in the described resource."@en;
  rdfs:label "has part"@en;
  rdfs:range <https://spec.edmcouncil.org/auto/ontology/VC/VehicleParts/VehiclePart> .

<http://data.europa.eu/m8g/StorageBatteryDevice> a owl:Class;
  rdfs:comment "An energy storage device capable of converting electric energy into chemical energy and back."@en;
  rdfs:label "Storage Battery Device"@en;
  rdfs:subClassOf <https://spec.edmcouncil.org/auto/ontology/VC/VehicleParts/VehiclePart>;
  owl:equivalentClass <https://smartdatamodels.org/dataModel.Battery/StorageBatteryDevice> .

<http://data.europa.eu/m8g/batteryType> a owl:ObjectProperty;
  rdfs:comment "Type of battery used."@en;
  rdfs:label "battery type"@en;
  rdfs:range skos:Concept;
  owl:equivalentProperty <https://smartdatamodels.org/dataModel.Battery/batteryType> .

<http://data.europa.eu/m8g/dateLastReported> a owl:DatatypeProperty;
  rdfs:comment "he last time when the device successfully reported data."@en;
  rdfs:label "date last reported"@en;
  rdfs:range xsd:dateTime;
  owl:equivalentProperty <https://smartdatamodels.org/dataModel.Battery/dateLastReported> .

<http://data.europa.eu/m8g/rechargeEnergySource> a owl:ObjectProperty;
  rdfs:comment "The type of power source of the battery."@en;
  rdfs:label "recharge energy source"@en;
  rdfs:range skos:Concept;
  owl:equivalentProperty <https://smartdatamodels.org/dataModel.Battery/rechargeEnergySource> .

<http://www.w3.org/ns/locn#geometry> a owl:ObjectProperty;
  rdfs:comment "Associates any Resource with the corresponding Geometry."@en;
  rdfs:label "geometry"@en;
  vann:usageNote """<p>Depending on how a geometry is encoded, the range of this property may be one of the following:
<ul>
 <li>- a literal (e.g., WKT - string literal -, GML, KML - XML literal)</li>
 <li>- a geometry class, as those defined in the OGC's GeoSPARQL specification, in the W3C's Basic Geo (WGS84 lat/long) vocabulary, and at schema.org;</li>
 <li>- geocoded URIs, as geo or GeoHash URIs, treated as URI references.</li>
</ul>

<p>
For interoperability reasons, it is recommended using one of the following:
<ul>
 <li>- Any geometry:
 <ul>
 <li> - WKT, GML, and RDF+WKT/GML, as per the GeoSPARQL specification.</li>
 <li> - KML (Keyhole Markup Language) - note that KML supports the following geometries only: point, line string, linear ring, and polygon.
 <li> - RDF as per the schema.org vocabulary (see classes schema:GeoCoordinates and schema:GeoShape).
 </ul>
 </li>
 <li>- Points: one of the above, or:
 <ul>
 <li> - RDF as per the W3C Basic Geo (WGS84 lat/long) vocabulary.</li>
 <li> - GeoHash URIs.</li>
 <li> - geo URIs.</li>
 </ul>
 </li>
</ul>
</p>"""@en;
  rdfs:range <http://www.w3.org/ns/locn#Geometry>;
  owl:equivalentProperty <https://smartdatamodels.org/dataModel.Battery/location>, <https://smartdatamodels.org/dataModel.Transportation/location> .

<http://data.europa.eu/m8g/nominalCapacity> a owl:ObjectProperty;
  rdfs:comment "Nominal Energy capacity."@en;
  rdfs:label "nominal capacity"@en;
  rdfs:range <http://qudt.org/schema/qudt/QuantityValue>;
  owl:equivalentProperty <https://smartdatamodels.org/dataModel.Battery/nominalCapacity> .

<http://data.europa.eu/m8g/nominalVoltage> a owl:ObjectProperty;
  rdfs:comment "Nominal battery voltage."@en;
  rdfs:label "nominal voltage"@en;
  rdfs:range <http://qudt.org/schema/qudt/QuantityValue>;
  owl:equivalentProperty <https://smartdatamodels.org/dataModel.Battery/nominalVoltage> .

<https://spec.edmcouncil.org/auto/ontology/VC/VehicleParts/VehiclePart> a owl:Class;
  rdfs:comment "Article the primary use of which is to improve, repair, replace, or serve as a component part of a vehicle."@en;
  rdfs:label "Vehicle Part"@en .

<http://data.europa.eu/m8g/createdOn> a owl:DatatypeProperty;
  rdfs:comment "Timestamp when the relation between the parent part and the child part was created."@en;
  rdfs:label "created on"@en;
  rdfs:range xsd:dateTime .

dct:identifier a owl:DatatypeProperty;
  rdfs:comment "Unique identifier of the entity"@en;
  rdfs:label "identifier"@en;
  rdfs:range xsd:string .

<http://data.europa.eu/m8g/lifecycleContext> a owl:ObjectProperty;
  rdfs:comment "The lifecycle context in which the child part was assembled into the parent part."@en;
  rdfs:label "lifecycle context"@en;
  rdfs:range skos:Concept .

dct:isPartOf a owl:ObjectProperty;
  rdfs:comment "Relationship between 2 branches where one is a component of the second."@en;
  rdfs:label "is part of"@en;
  rdfs:range <http://data.europa.eu/m8g/ElectricCar>;
  owl:equivalentProperty <https://www.w3.org/TR/vsso-core/#partOfVehicle> .

<http://data.europa.eu/m8g/quantity> a owl:ObjectProperty;
  rdfs:comment "Quantity of which the child part is assembled into the parent part."@en;
  rdfs:label "quantity"@en;
  rdfs:range <http://qudt.org/schema/qudt/QuantityValue> .

<https://spec.edmcouncil.org/auto/ontology/VS/VehicleSignals/VehicleSensor> a owl:Class;
  rdfs:comment "A device which monitors a vehicle part."@en;
  rdfs:label "Vehicle Sensor"@en;
  rdfs:subClassOf <https://spec.edmcouncil.org/auto/ontology/VC/VehicleParts/VehiclePart> .

<http://qudt.org/schema/qudt/QuantityValue> a owl:Class;
  rdfs:comment "A Quantity Value expresses the magnitude and kind of a quantity and is given by the product of a numerical value and a unit of measure."@en;
  rdfs:label "Quantity Value"@en .

<http://qudt.org/schema/qudt/unit> a owl:ObjectProperty;
  rdfs:comment "Unit of Measurement for the quantity of serialized objects."@en;
  rdfs:label "unit of measure"@en;
  rdfs:range <http://qudt.org/schema/qudt/Unit> .

<http://qudt.org/schema/qudt/value> a owl:DatatypeProperty;
  rdfs:comment "A property to relate an observable thing with a value of any kind."@en;
  rdfs:label "value"@en;
  rdfs:range xsd:double;
  owl:equivalentClass <https://schema.org/QuantitativeValue>, <https://spec.edmcouncil.org/auto/ontology/MO/MiddleOntology/QuantitativeValue>,
    """bamm:io.catenax.assembly_part_relationship:1.1.1#QuantityT
ype: http://www.w3.org/2001/XMLSchema#string"""@en .

<https://smartdatamodels.org/dataModel.Battery/StorageBatteryMeasurement> a owl:Class;
  rdfs:comment "A report genereated on the battery."@en;
  rdfs:label "Storage Battery Measurement"@en .

<http://data.europa.eu/m8g/dateObserved> a owl:DatatypeProperty;
  rdfs:comment "The date time in which the measurement was taken."@en;
  rdfs:label "date observed"@en;
  rdfs:range xsd:dateTime;
  owl:equivalentProperty <https://smartdatamodels.org/dataModel.Battery/dateObserved> .

<http://data.europa.eu/m8g/stateOfCharge> a owl:ObjectProperty;
  rdfs:comment "The ratio between the remaining and the current capacities."@en;
  rdfs:label "state of charge"@en;
  rdfs:range <http://qudt.org/schema/qudt/QuantityValue>;
  owl:equivalentProperty <https://smartdatamodels.org/dataModel.Battery/stateOfCharge> .

<http://data.europa.eu/m8g/stateOfHealth> a owl:ObjectProperty;
  rdfs:comment "The ratio between the maximum amount of charge that a fully charged battery can provide under its nominal discharge regime, and its nominal capacity."@en;
  rdfs:label "state of health"@en;
  rdfs:range <http://qudt.org/schema/qudt/QuantityValue>;
  owl:equivalentProperty <https://smartdatamodels.org/dataModel.Battery/stateOfHealth> .

<https://smartdatamodels.org/dataModel.Transportation/EVChargingStation> a owl:Class;
  rdfs:comment "Infrastructure that supplies electric energy for the recharging of electric vehicles."@en;
  rdfs:label "Charging Station"@en .

<http://data.europa.eu/m8g/allowedVehicleType> a owl:ObjectProperty;
  rdfs:comment "Vehicle type(s) which can be charged."@en;
  rdfs:label "allowed vehicle type"@en;
  rdfs:range skos:Concept;
  owl:equivalentProperty <https://smartdatamodels.org/dataModel.Transportation/allowedVehicleType> .

<http://data.europa.eu/m8g/capacity> a owl:DatatypeProperty;
  rdfs:comment "The total number of vehicles which can be charged at the same time. The total number of sockets can be higher."@en;
  rdfs:label "capacity"@en;
  rdfs:range xsd:integer;
  owl:equivalentProperty <https://smartdatamodels.org/dataModel.Transportation/capacity> .

rdfs:label a owl:DatatypeProperty;
  rdfs:comment "The name of the charging station"@en;
  rdfs:label "name"@en;
  rdfs:range rdf:langString;
  owl:equivalentProperty <https://smartdatamodels.org/dataModel.Transportation/name> .

<http://data.europa.eu/m8g/socketType> a owl:ObjectProperty;
  rdfs:comment "The type of sockets offered by this station."@en;
  rdfs:label "socket type"@en;
  rdfs:range skos:Concept;
  owl:equivalentProperty <https://smartdatamodels.org/dataModel.Transportation/socketType> .

<http://data.europa.eu/m8g/address> a owl:ObjectProperty;
  rdfs:comment "Associates any Resource with the corresponding Address."@en;
  rdfs:label "address"@en;
  vann:usageNote "Asserting the address relationship implies that the Resource has an Address."@en;
  rdfs:range <http://www.w3.org/ns/locn#Address>;
  owl:equivalentProperty <https://smartdatamodels.org/dataModel.Transportation/address> .